Progress on critbit

LiveVerif/src/LiveVerifExamples/critbit.v
@@ -43,7 +43,59 @@ Context {consts: malloc_constants}.
 Context {word_map: map.map word word}.
 Context {word_map_ok: map.ok word_map}.
 
-Definition prefix_bits (n: Z) (w: word) := word.and (word.not (/[-1] ^<< /[n])) w.
+Definition prefix_bits (n: Z) (w: word) :=
+  if n =? 32 then w else word.and (word.not (/[-1] ^<< /[n])) w.
+
+Lemma testbit_1 : forall i : Z, Z.testbit 1 i = (i =? 0).
+Proof.
+  intros. unfold Z.testbit. destruct i; reflexivity.
+Qed.
+
+Ltac unfold_bits_step :=
+  match goal with
+  | |- context[ ?X mod 2 ^ 32 ] =>
+      let Hb := fresh "Hb" in assert (Hb: 0 <= X < 2 ^ 32); [ lia | ];
+                              rewrite (Z.mod_small X (2 ^ 32) Hb); clear Hb
+  | H: context[ ?X mod 2 ^ 32 ] |- _ =>
+      let Hb := fresh "Hb" in assert (Hb: 0 <= X < 2 ^ 32); [ ZnWords | ];
+                              rewrite (Z.mod_small X (2 ^ 32) Hb) in H; clear Hb
+  | _ => rewrite word.unsigned_and in *
+  | _ => rewrite word.unsigned_or in *
+  | _ => rewrite word.unsigned_not in *
+  | _ => rewrite word.unsigned_slu; [ | ZnWords ]
+  | _ => rewrite word.unsigned_sru; [ | ZnWords ]
+  | H: context[ \[word.slu _ _] ] |- _ => rewrite word.unsigned_slu in H; [ | ZnWords ]
+  | H: context[ \[word.sru _ _] ] |- _ => rewrite word.unsigned_sru in H; [ | ZnWords ]
+  | _ => rewrite word.unsigned_of_Z in *
+  | _ => rewrite <- Z.land_ones; [ | lia ]
+  | _ => rewrite Z.testbit_ones; [ | lia ]
+  | _ => rewrite Z.land_spec in *
+  | _ => rewrite Z.lor_spec in *
+  | _ => rewrite bitblast.Z.shiftl_spec' in *
+  | _ => rewrite bitblast.Z.shiftr_spec' in *
+  | _ => rewrite bitblast.Z.lnot_spec' in *
+  | _ => rewrite Z.bits_0 in *
+  | _ => rewrite bitblast.Z.testbit_minus1' in *
+  | _ => rewrite testbit_1 in *
+  | H: context[ word.wrap ] |- _ => unfold word.wrap in H
+  | _ => unfold word.wrap
+  end.
+
+Ltac unfold_bits := repeat unfold_bits_step.
+
+Lemma prefix_bits_is_modulo : forall (n: Z) (w: word),
+    0 <= n <= 32 -> prefix_bits n w = /[\[w] mod (2^n)].
+Proof.
+  (* maybe we could use the bitblast tactic here? *)
+  intros. apply word.unsigned_inj. apply Z.bits_inj. unfold Z.eqf.
+  intros. assert (n = 32 \/ n < 32).
+  lia. destruct H0; unfold prefix_bits;
+    [ assert (Hc: n =? 32 = true); [ lia | ] | assert (Hc: n =? 32 = false); [ lia | ] ];
+    rewrite Hc; unfold_bits; (replace (\[w]) with (\[w] mod 2 ^ 32); [ | ZnWords ]);
+    unfold_bits; destruct (Z.testbit \[w] n0); lia.
+  (* invoking unfold_bits for a second time because that adds the information
+     that testbit \[w] is non-zero only for indices 0 to 31 *)
+Qed.
 
 Record prefix: Type := {
     length: Z;
@@ -69,17 +121,86 @@ Definition append_1 (p: prefix) :=
 
 Definition full_prefix (k: word) := {| length := 32; bits := k |}.
 
+Definition is_prefix_key (p: prefix) (k: word) := is_prefix p (full_prefix k).
+
+Ltac f_apply f H :=
+  match type of H with
+  | ?lhs = ?rhs =>
+      let h := fresh "H" in assert (h: f lhs = f rhs); [ rewrite H; reflexivity | ];
+                            cbv beta in h; clear H; rename h into H
+  end.
+
+Ltac prove_is_prefix_append_x :=
+  intros;
+  unfold is_prefix; unfold append_0; unfold append_1; unfold bit_at;
+  unfold canonic_bits; unfold prefix_bits;
+  split; simpl; [ lia | ];
+  replace (length _ =? 32) with false; [ | lia ];
+  apply word.unsigned_inj; apply Z.bits_inj; unfold Z.eqf;
+  intros; unfold_bits; destruct (Z.testbit \[bits _]); lia.
+
+Lemma is_prefix_append_0 : forall p, 0 <= length p < 32 -> is_prefix p (append_0 p).
+Proof.
+  prove_is_prefix_append_x.
+Qed.
+
+Lemma is_prefix_append_1 : forall p, 0 <= length p < 32 -> is_prefix p (append_1 p).
+Proof.
+  prove_is_prefix_append_x.
+Qed.
+
+Lemma is_prefix_trans : forall p1 p2 p3,
+    0 <= length p1 <= 32 -> 0 <= length p2 <= 32 -> 0 <= length p3 <= 32 ->
+    is_prefix p1 p2 -> is_prefix p2 p3 -> is_prefix p1 p3.
+Proof.
+  intros. unfold is_prefix in *. split. lia. destruct H2. destruct H3.
+  rewrite prefix_bits_is_modulo in *; try lia.
+  rewrite prefix_bits_is_modulo in *; try lia.
+  f_equal.
+  Ltac extract_equality H :=
+    let Hres := fresh "H" in
+    eassert (Hres: \[ ?[a] ] = \[ ?[b] ]);
+    [ apply f_equal; exact H | ];
+    repeat rewrite word.unsigned_of_Z in Hres; unfold word.wrap in Hres;
+    rewrite (Zmod_small _ (2 ^ 32)) in Hres;
+    (* infinite loop if I use repeat rewrite here?! *)
+    rewrite (Zmod_small _ (2 ^ 32)) in Hres;
+    clear H; rename Hres into H.
+  extract_equality H4.
+  extract_equality H5.
+  f_apply (fun n => n mod (2 ^ length p1)) H5.
+  replace (length p2) with (length p1 + (length p2 - length p1)) in H5; [ | lia].
+  rewrite Z.pow_add_r in H5. rewrite Z.rem_mul_r in H5. rewrite Z.rem_mul_r in H5.
+  rewrite Z.mul_comm in H5. rewrite Z_mod_plus_full in H5.
+  rewrite Z.mul_comm in H5. rewrite Z_mod_plus_full in H5.
+  repeat rewrite Zmod_mod in H5. congruence.
+  all: try lia.
+  all: match goal with | |- context[?a mod ?b] => assert (0 <= a mod b < b);
+    [ apply Z_mod_lt; lia | ]; assert (b <= 2 ^ 32); [ apply Z.pow_le_mono_r; lia | ]
+       end; lia.
+Qed.
+
+Lemma is_prefix_key_trans : forall p1 p2 k,
+    0 <= length p1 <= 32 -> 0 <= length p2 <= 32 ->
+    is_prefix p1 p2 -> is_prefix_key p2 k -> is_prefix_key p1 k.
+Proof.
+  intros. unfold is_prefix_key in *. eapply is_prefix_trans. all: cycle 3.
+  eassumption. assumption. 3: simpl. all: lia.
+Qed.
+
+(* no need to use word (record) for ghost: might use positive *)
 Fixpoint cbt' (sk: tree_skeleton) (p: prefix) (c: word_map) (a: word): mem -> Prop :=
   match sk with
     | Leaf => ex1 (fun k: word => ex1 (fun v: word =>
         <{ * emp (a <> /[0])
-           * emp (c = map.singleton k v)
-           * emp (p = full_prefix k)
+           * freeable 12 a
            * <{ + uint 32 (-1)
                 + uintptr k
-                + uintptr v }> a }>))
+                + uintptr v }> a
+           * emp (p = full_prefix k)
+           * emp (c = map.singleton k v) }>))
   | Node skL skR => ex1 (fun aL: word => ex1 (fun pL: prefix => ex1 (fun cL: word_map =>
-     ex1 (fun ix: Z => ex1 (fun aR: word => ex1 (fun pR: prefix => ex1 (fun cR: word_map
+     ex1 (fun aR: word => ex1 (fun pR: prefix => ex1 (fun cR: word_map
           =>
           <{ * emp (a <> /[0])
              * freeable 12 a
@@ -92,7 +213,7 @@ Fixpoint cbt' (sk: tree_skeleton) (p: prefix) (c: word_map) (a: word): mem -> Pr
              * emp (is_canonic p)
              * emp (is_prefix (append_0 p) pL)
              * emp (is_prefix (append_1 p) pR)
-             * emp (map.split c cL cR) }>)))))))
+             * emp (map.split c cL cR) }>))))))
   end.
 
 Definition nncbt (c: word_map) (a: word): mem -> Prop :=
@@ -103,6 +224,7 @@ Definition nncbt (c: word_map) (a: word): mem -> Prop :=
    - pointing to the CBT root node *)
 Definition cbt (c: word_map) (a: word): mem -> Prop :=
   or1 (nncbt c a) (emp (c = map.empty /\ a = /[0])).
+
 
 #[export] Instance spec_of_cbt_init: fnspec :=                              .**/
 
@@ -120,10 +242,24 @@ unfold cbt. exists (map.empty). exists m. step. apply map.split_empty_l.
 step. step. right. unfold emp. tauto. tauto.
 Qed.
 
+Lemma purify_cbt' :
+  forall sk p c a, purify (cbt' sk p c a) (a <> /[0] /\ 0 <= length p <= 32).
+Proof.
+  unfold purify. intros. unfold cbt' in H. destruct sk;
+  [ destruct H as [k [v [m0 [m1 [_ H]]]]] |
+    destruct H as [aL [pL [cL [aR [pR [cR [m0 [m1[_ H]]]]]]]]] ]; steps.
+Qed.
+
+Lemma purify_wand : forall (P Q: mem -> Prop), purify (wand P Q) True.
+Proof. unfold purify. auto. Qed.
 
 #[local] Hint Extern 1 (cannot_purify (cbt' _ _ _))
       => constructor : suppressed_warnings.
+#[local] Hint Extern 1 (cannot_purify (cbt' _ _ _ _))
+      => constructor : suppressed_warnings.
 #[local] Hint Extern 1 (cannot_purify (cbt _ _))
+      => constructor : suppressed_warnings.
+#[local] Hint Extern 1 (cannot_purify (wand _ _))
       => constructor : suppressed_warnings.
 #[local] Hint Extern 1 (cannot_purify (nncbt _ _))
       => constructor : suppressed_warnings.
@@ -131,8 +267,35 @@ Qed.
       => constructor : suppressed_warnings.
 #[local] Hint Extern 1 (cannot_purify (or1 _ _))
       => constructor : suppressed_warnings.
+#[local] Hint Extern 1 (PredicateSize_not_found (wand _))
+      => constructor : suppressed_warnings.
 
 #[local] Hint Unfold cbt : heapletwise_always_unfold.
+#[local] Hint Unfold nncbt : heapletwise_always_unfold.
+
+Hint Resolve purify_cbt' : purify.
+Hint Resolve purify_wand : purify.
+Print HintDb purify.
+
+Lemma cbt_key_has_prefix : forall (sk: tree_skeleton) (p: prefix) (c: word_map) (a: word) (m: mem) (k: word),
+    cbt' sk p c a m -> map.get c k <> None -> is_prefix_key p k.
+Proof.
+  induction sk.
+  - intros. unfold cbt' in H. steps.
+  - intros. simpl in H. steps. apply split_du in H11. unfold map.split in H11.
+    destruct H11. destruct (map.get c k) eqn:E; [ | tauto ]. clear H0.
+    subst c. epose proof (map.putmany_spec cL cR k). destruct H.
+    destruct H as [v [H H']]. clear IHsk1. pose proof H5.
+    eapply IHsk2 with (k:=k) in H5.
+    eapply is_prefix_key_trans. lia. 3: eassumption. assumption.
+    eapply is_prefix_trans. lia. 4: eassumption. simpl. lia. lia.
+    eapply is_prefix_append_1. lia. rewrite H. discriminate.
+    clear IHsk2. eapply IHsk1 with (k:=k) in H4.
+    eapply is_prefix_key_trans. lia. 3: eassumption. lia.
+    eapply is_prefix_trans. lia. 4: eassumption.
+    simpl. lia. lia. eapply is_prefix_append_0. lia. destruct H.
+    rewrite E in H0. rewrite <- H0. discriminate.
+Qed.
 
 #[export] Instance spec_of_dummy: fnspec := .**/
 uintptr_t dummy( ) /**#
@@ -148,27 +311,305 @@ Check .**/ void dummy( ) /**#
 Check spec_of_dummy : Semantics.env -> Prop.
 Print spec_of_dummy.
 
+(* observation: if A and B both can't be purified, purify_rec fails on sep A B, but
+not on sep A P or sep P B, where P can be purified *)
+
+(*
+loop invariant (holds both before, during, and after loop):
+variables p (current CBT pointer), cc (current CBT content), sk (current CBT skeleton)
+memory: nncbt cc p * wand (nncbt cc p) (nncb c tp) * R
+additional condition: map.get c k = None <-> map.get cc k
+*)
+
+Require Import bedrock2.PurifySep.
+(*
+Ltac is_var_b x ::=
+  match constr:(Set) with
+  | _ => let __ := match constr:(Set) with
+                   | _ => idtac "is_var_b is getting called with" x; is_var x
+                   end in
+         constr:(true)
+  | _ => constr:(false)
+  end.
+*)
+
+Lemma wand_trans : forall (P Q R : mem -> Prop),
+    impl1 <{ * wand P Q * wand Q R }> (wand P R).
+Proof.
+  intros. unfold impl1. intros. unfold sep in H. destruct H as [mp [mq [H1 [H2 H3]]]].
+  unfold wand in *. intros. unfold map.split in *. destruct H1. destruct H.
+  subst x. apply map.disjoint_putmany_l in H5. destruct H5.
+  eapply H3 with (m1 := map.putmany m1 mp). split. subst m2.
+  rewrite map.putmany_comm. rewrite map.putmany_assoc. rewrite map.putmany_comm.
+  reflexivity. apply map.disjoint_putmany_l. split. apply map.disjoint_comm.
+  assumption. assumption. apply map.disjoint_putmany_l. split; assumption.
+  apply map.disjoint_putmany_r. split. assumption. apply map.disjoint_comm.
+  assumption. eapply H2. split. eapply map.putmany_comm. apply map.disjoint_comm.
+  assumption. assumption. assumption.
+Qed.
+
+Lemma wand_ex_r : forall {A: Type} (P : mem -> Prop) (Q: A -> mem -> Prop),
+    impl1 (ex1 (fun x => wand P (Q x))) (wand P (ex1 Q)).
+Proof.
+Admitted.
+
+Lemma du_def_split : forall (m m1 : mem) (mm: mmap mem),
+    mm \*/ m1 = m -> exists m2 : mem, mm = m2 /\ map.split m m2 m1.
+Proof.
+  intros. pose proof H. unfold "\*/" in H0. destruct mm eqn:E. exists m0.
+  split. reflexivity. apply split_du. assumption. discriminate.
+Qed.
+
+
+Lemma append_0_prefix : forall (p : prefix) (k : word),
+    0 <= length p <= 31 -> is_prefix_key (append_0 p) k ->
+    word.and (k ^>> /[length p]) /[1] = /[0].
+Proof.
+Admitted.
+  (*
+  (*
+  intros p k. unfold is_prefix_key. unfold is_prefix.
+  unfold full_prefix. simpl. unfold canonic_bits. unfold prefix_bits.  *)
+  intros. unfold is_prefix_key in *. unfold is_prefix in *. simpl in *.
+  unfold canonic_bits in *. unfold prefix_bits in *.
+  destruct (length p + 1 =? 32) eqn:E. destruct (length p =? 32) eqn:E2.
+  lia. apply word.unsigned_inj. ZnWords_pre. apply Z.bits_inj. unfold Z.eqf. destruct H0.
+  subst k. intros. unfold_bits. lia. destruct (length p =? 32) eqn:E2. lia.
+  apply word.unsigned_inj. apply Z.bits_inj. unfold Z.eqf. destruct H0.
+  intros. f_apply (fun x => Z.testbit \[x] (n + length p)) H1. unfold_bits.
+  rewrite Z.land_spec.
+  apply word.unsigned_inj. apply Z.bits_inj. unfold Z.eqf. destruct H.
+  intros. f_apply (fun x => \[x]) H0. unfold_bits.
+  rewrite Z.land_spec in
+  destruct (Z.testbit 0 n). f_apply (fun x => \[x]) H0. unfold_bits.
+  unfold_bits. destruct
+   *)
+
+Lemma append_1_prefix : forall (p : prefix) (k : word),
+    0 <= length p <= 31 -> is_prefix_key (append_1 p) k ->
+    word.and (k ^>> /[length p]) /[1] = /[1].
+Proof.
+Admitted.
+
+(*
+Lemma du_on_sep : forall (m m1 m2: mem) (P Q : mem -> Prop), P m1 -> Q m2 -> mmap.du m1 m2 = m -> sep P Q m.
+Proof.
+  steps. change (P m1) with (m1 |= P) in H.
+  change (Q m2) with (m2 |= Q) in H0. step. step. step.
+  change (m1 \*/ m2) with
+  (interp_mem_tree (NDisjointUnion (NLeaf m1) (NLeaf m2))). apply cancel_head.
+*)
+
+
+Ltac evar_dbg ev val := eassert (ev = val); reflexivity.
+
+Local Hint Extern 1 (PredicateSize (cbt' ?sk)) => exact 12 : typeclass_instances.
+
 #[export] Instance spec_of_cbt_best_leaf: fnspec :=                             .**/
+
 
 uintptr_t cbt_best_leaf(uintptr_t tp, uintptr_t k) /**#
   ghost_args := (c: word_map) (R: mem -> Prop);
   requires t m := <{ * nncbt c tp
                      * R }> m;
-  ensures t' m' res := t' = t /\ ex1 (fun k' => ex1 (fun v' =>
+  ensures t' m' res := t' = t (* /\ ex1 (fun k' => ex1 (fun v' =>
                   let leaf := cbt' Leaf (full_prefix k') (map.singleton k' v') res in
                         <{ * leaf
                            * wand leaf (nncbt c tp)
-                           * emp (k <> k' <-> map.get c k = None)}> )) m' #**/     /**.
+                           * emp (k <> k' <-> map.get c k = None)}> )) m' *) #**/     /**.
 Derive cbt_best_leaf SuchThat (fun_correct! cbt_best_leaf) As cbt_best_leaf_ok.  .**/
 {                                                                            /**. .**/
-  uintptr_t p = tp;                                                            /**.
-  loop invariant above Def0. .**/
+  uintptr_t p = tp;                                                          /**.
+  rename p' into pr. move H0 at bottom. move sk at bottom. rewrite <- Def0 in H0.
+  move m0 at bottom. remember c as cc.
+  prove (m0 |= sep (cbt' sk pr cc p) (wand (cbt' sk pr cc p) (nncbt c tp))).
+  subst cc. unfold nncbt. unfold sep. unfold "|=". exists m0. exists map.empty.
+  split. apply map.split_empty_r. reflexivity. split. assumption. unfold wand.
+  intros. eexists. eexists. apply map.split_empty_l in H. subst p. subst m3.
+  (* use a lemma to get the wand *)
+  eassumption.
+  prove (map.get c k = None <-> map.get cc k = None). subst cc. reflexivity.
+  clear H0.
+  clear Heqcc. move cc before pr.
+  loop invariant above p. clear Def0.
+Ltac log_packaged_context P ::= idtac P.
+.**/
+  while (load32(p) != -1) /* decreases sk */ { /*?.
+
+  subst v. destruct sk. simpl cbt' in *. steps. simpl cbt' in *.
+  step. step. step. step. step. step. step. step. step. step. step.
+  step. step. step. step. step. step. step. step. step. step. step. step. step.
+  step. step. step. step. step. step. step. step. step. step. step. step. step.
+  constructor. constructor. constructor. step. step. step; [ | trivial]. step.
+  step. step. step. Show Existentials.
+  .**/
+  (* without "== 1", not supported in one of the tactics *)
+  if (((k >> load32(p)) & 1) == 1) { /**.
+  (* to debug evar instantiation failure: write an ltac snippet to get the evar into
+  an ltac variable; write assert (myevar = valueImtryingtoassign). reflexivity. ->
+  gives better error message *)
+  (* continue with this function; try another CBT function; implement delete (in C) *)
+  .**/
+    p = load(p + 8);   /**. .**/
+  } /**. unfold canceling. unfold seps.
+  step. step. step.
+  unzify. (* write and use lemmas about wand and ex1 *)
+  eapply wand_trans. eassert (mmap.Def m4 = _ \*/ m3). rewrite <- D.
+  rewrite mmap.du_assoc. rewrite mmap.du_comm with (p := m3).
+  rewrite <- mmap.du_assoc. reflexivity.
+  symmetry in H1. destruct ((m2 \*/ m5) \*/ m1) eqn:E; [ | discriminate].
+  apply split_du in H1. unfold map.split in H1. destruct H1. rewrite H1.
+  apply sep_from_disjointb. apply map.disjointb_spec. assumption. 2: eassumption.
+  clear H5 H15 H1 D m4 m3.
+  (* use exists x. A -> B    ->    A -> exists x. B lemma for wands here *)
+  unfold wand. intros. exists aL. exists pL. exists cL. exists p. exists pR. exists cR.
+  step. step. step. step. step. step. step. step. unfold canceling.
+  split; [ | trivial ]. intros. injection H15 as H15. subst m.
+  unfold seps. replace m3 with (map.putmany m3 map.empty). apply sep_from_disjointb.
+  apply map.disjointb_spec. apply map.disjoint_empty_r. assumption.
+  repeat rewrite sep_emp_l. step. step. step. step. step. step. step. step.
+  apply split_du in H14. unfold emp. split; trivial. apply map.putmany_empty_r.
+  split; [ | trivial ]. rewrite H4. split. apply split_du in H14.
+  unfold map.split in H14. destruct H14. subst cc. intros.
+  apply map.invert_get_putmany_None in H1. destruct H1. assumption.
+  step. destruct (map.get cc k) eqn:E; [ exfalso | trivial ]. apply split_du in H14.
+  apply map.get_split with (k:=k) in H14. destruct H14; destruct H14.
+  rewrite H14 in E. apply cbt_key_has_prefix with (k:=k) in H7.
+  eapply is_prefix_key_trans in H11. 4: eassumption. apply append_0_prefix in H11.
+  rewrite H11 in H. ZnWords. step. unfold append_0. simpl. step. step. congruence.
+  congruence. .**/
+  else { /**. .**/
+    p = load(p + 4);  /**. .**/
+  } /**. unfold canceling. unfold seps. step. step. step. eapply wand_trans.
+  unfold seps. apply sep_comm. step. step. unfold canceling. step. step. step.
+  unfold seps. apply wand_ex_r. step. apply wand_ex_r. step. apply wand_ex_r.
+  step. apply wand_ex_r. step. apply wand_ex_r. step. apply wand_ex_r. step.
+  unfold wand. intros. step. step. step. step. step. step. step.
+  change (cbt' sk1 pL cL p m4) with (m4 |= cbt' sk1 pL cL p) in H15. step. step.
+  step. step. step. step. step. step. step. step. step. rewrite <- split_du in H14.
+  assumption. step. step. step. step. rewrite H4. clear H4 H5.
+  split. step.
+  apply split_du in H14. unfold map.split in H14. destruct H14. subst cc.
+  apply map.invert_get_putmany_None in H1. step. assumption. step.
+  destruct (map.get cc k) eqn:E; [ exfalso | trivial ]. apply split_du in H14.
+  apply map.get_split with (k:=k) in H14. destruct H14; step. congruence.
+  rewrite H4p0 in E. apply cbt_key_has_prefix with (k:=k) in H8.
+  eapply is_prefix_key_trans in H12. 4: eassumption. apply append_1_prefix in H12.
+  congruence. step. unfold append_1. simpl. step. step. congruence. step. .**/
+  } /**. .**/
+  return p; /**.
+steps.
+  step. .**/
+  } /**. .**/
+  return p; /**.
+ step. step. step. step. step. step. step. step. step.
+  step. step. unfold cbt'. unfold split_range_from_hyp. unfold canceling.
+  step. unfold cbt' in H3. step. step. step. step. step. step. step. step. step.
+  step. step. step. step. unfold cbt' in H3. step. step. step. step. step. step.
+  step. step. step. step. step. Unshelve. exact nil. exact cmd.skip. .**/
+  } /**.
+  apply cbt_key_has_prefix with (k:=k) in H6. eapply is_prefix_key_trans in H12.
+
+  assu
+
+
+  step. rewrite sep_co
+  eassert (mmap.Def m4 = _ \*/ m3). rewrite <- D. rewrite mmap.du_assoc.
+  rewrite mmap.du_comm with (p := m3). rewrite <- mmap.du_assoc. reflexivity.
+  destruct ((m2 \*/ m6) \*/ m1) eqn:E; [ | discriminate ]. clear E D. symmetry in H1.
+  step.
+  eassert (m |= _). admit.
+  apply split_du in H1. unfold map.split in H1
+  apply wand_ex_r. step.
+  apply wand_ex_r. step.
+
+
+
+  step. step. step. step. step.
+  step. step. step. step. step. step. step. step. step. step. step. step. step. step.
+  step. step. step. step. step. step. step. step. step. step. step. step.
+  apply du_def_split in H1. destruct H1 as [m7 H1].
+  unfold "\*/" in H1.
+  destruct (mmap.of_option (map.du m2 m5)) eqn:E.
+  destruct (mmap.of_option (map.du m m1)) eqn:E2.
+  eassert (map.split m4 _ m3). instantiate (1 := m7).
+  unfold map.du in H1. destruct (map.disjointb m7 m3). simpl in H1. injection H1 as H1.
+  subst m4. apply map.split_disjoint_putmany. Check (mmap.Def m).
+  Set Printing Coercions. Chinstantiate (1 := ?[mymy]).
+  (* instantiate (mymy := m7). *) Check ?Q. evar_dbg ?mymy m7.
+  step. step. step. step. step. step. step.
+  constructor. constructor. instantiate (1 := k).
+  unfold WeakestPrecondition.dexpr. simpl. subst l. simpl.
+  unfold WeakestPrecondition.get. exists k. simpl. step.
+  unfold SortedList.lookup. simpl. step. step. step. step. step.
+  instantiate (8 := p0). constructor. constructor.
+  unfold WeakestPrecondition.dexpr. simpl. subst l. simpl.
+  unfold WeakestPrecondition.get. exists p0. simpl. step.
+  unfold SortedList.lookup. simpl. step. step. step. step. step.
+  unfold canceling. step. step. step.
+
+  destruct v.
+
+  unfold cbt' in H4. step. step. step. step. step. step. step. step.
+  step. step. step.
+
+  simpl in H4. step. step. step. step. step. step. step. step.
+  step. step. step. step. step. step. step. step. step. step. step. step. step.
+  step. step. unfold seps. step. step. step. step. step. step. step. step.
+  step. step. step. step. step. step. step. step.
+
+  (* assignment in if-branch *)
+  eapply (wp_set) with (x := "p") (e := (live_expr:(load32(p + 8)))).
+  step. step. constructor. constructor. instantiate (1 := p0).
+  unfold WeakestPrecondition.dexpr. simpl. subst l. simpl.
+  unfold WeakestPrecondition.get. exists p0. simpl. step.
+  unfold SortedList.lookup. simpl. step. step. step. step. step.
+
+  destruct v.
+
+  unfold cbt' in H4. step. step. step. step. step. step. step. step. step.
+  step. step. step. step. step. step. step.
+
+  simpl in H4. step. step. step. step. step. step. step. step. step.
+  step. step. step. step. step. step. step. step. step. step. step. step.
+  step. step. step. step. step. step. step. step. step. step. step.
+  instantiate (2 := \[aR]). Check \[aR]. Checstep. step. step. step. step. step. step.
+  instantiate (8 :
+
+  .**/
+    kb = 1;                     /**.
+
+  (* leaf case *)
+  unfold cbt' in H4. step. step. step. step. step. step.
+  step. step. step. step. step.
+
+  split.
+  assumption. split. assumption. split. assumption. reflexivity.
+  eauto with wf_of_type. intros. destruct v. exists false. destruct H0. destruct H0.
+  destruct H0. destruct H0. destruct H0. destruct H0. destruct H3. destruct H4.
+  destruct H5. subst l. destruct H0. destruct H0. destruct H0. destruct H6.
+  apply mk_dexpr_bool3 with (/[0]). constructor. step. step.
+  unfold "|=" in H. step. step. step. stepassert (emp True m0).
+  admit. purify_hyp H8. unfold "|=" in H. purify_
+  purify H4. step. bedrock2.PurifySep.purify H.
+  Ltac purified_hyp_of_pred ::= fail 10000. step.
+  **/
+  if (k & 1 << load32(p)) { /**.
+  destruct "\*/" in D
+  eapply (wp_while_tailrec_with_done_flag measure0 (sk, cc, p, pr, R) cond).
+  eauto with wf_of_type.
+    { Ltac log_packaged_context P ::= idtac P.
+    package_heapletwise_context. }
+  {       collect_heaplets_into_one_sepclause.
+
+  loop invariant above Def0. .**/ *) Abort. (*
   while (load32(p) != 0) /* decreases (1) */ {                        /**.
   (* the termination measure should be the tree skeleton. How do we get
      the skeleton out of p? *)
   (* -> ?apply the while rule manually? *)
-Abort.
-
+Abort. *)
+(* use result pointer *)
+(* keep a log *)
 #[export] Instance spec_of_cbt_lookup: fnspec :=                                .**/
 (* parameter "d" for "default" *)
 uintptr_t cbt_lookup(uintptr_t tp, uintptr_t k, uintptr_t d) /**#
@@ -184,11 +625,11 @@ Derive cbt_lookup SuchThat (fun_correct! cbt_lookup) As cbt_lookup_ok.          
   if (tp == NULL) /* split */ {                                             /**. .**/
     return d;                                                               /**. .**/
   }                                                                         /*?.
-  step. step. step. step. step.  destruct H0. destruct H0. destruct H0.
-  destruct x; simpl in H0. step. step. step. step. step. step. step. step.
+  step. step. step. step. step.  destruct H0. unfold nncbt in H0. step. step.
+  destruct sk; simpl in H0. step. step. step. step. step. step. step. step.
   step. step. step. step. step. step. step. step. step. step. step. step.
   step. step. step. step. step. step. step. step. step. step. step. step.
-  step. step. step. step. step. step. subst c. rewrite map.get_empty. step.
+  step. step. step. step. step. subst c. rewrite map.get_empty. step.
   subst tp. steps.                                                               .**/
   else {                                                                    /**.
   Abort.
@@ -196,12 +637,11 @@ Derive cbt_lookup SuchThat (fun_correct! cbt_lookup) As cbt_lookup_ok.          
 #[export] Instance spec_of_cbt_insert: fnspec :=                                  .**/
 
 uintptr_t cbt_insert(uintptr_t tp, uintptr_t k, uintptr_t v) /**#
-  ghost_args := (c c': word_map) (R: mem -> Prop);
+  ghost_args := (c: word_map) (R: mem -> Prop);
   requires t m := <{ * cbt c tp
                      * R }> m;
   ensures t' m' res := t' = t
-           /\ <{ * emp (map.put c k v = c') (* should this really be equality? *)
-                 * cbt c' res
+           /\ <{ * cbt (map.put c k v) res
                  * R }> m'        #**/                                      /**.
 Derive cbt_insert SuchThat (fun_correct! cbt_insert) As cbt_insert_ok.
 (* TODO: implement & prove *)
